wip

fstar-helpers/minicore/src/abstractions/bit.rs
@@ -68,9 +68,12 @@ impl From<bool> for Bit {
 }
 
 /// A trait for types that represent machine integers.
+#[hax_lib::attributes]
 pub trait MachineInteger {
     /// The size of this integer type in bits.
-    const BITS: u32;
+    #[hax_lib::requires(true)]
+    #[hax_lib::ensures(|bits| bits >= 8)]
+    fn bits() -> u32;
 
     /// The signedness of this integer type.
     const SIGNED: bool;
@@ -79,7 +82,7 @@ pub trait MachineInteger {
 macro_rules! generate_machine_integer_impls {
     ($($ty:ident),*) => {
         $(#[hax_lib::exclude]impl MachineInteger for $ty {
-            const BITS: u32 = $ty::BITS;
+            fn bits() -> u32 { $ty::BITS }
             #[allow(unused_comparisons)]
             const SIGNED: bool = $ty::MIN < 0;
         })*
@@ -90,7 +93,10 @@ generate_machine_integer_impls!(u8, u16, u32, u64, u128, i8, i16, i32, i64, i128
 #[hax_lib::fstar::replace(
     r"
 instance impl_MachineInteger_poly (t: inttype): t_MachineInteger (int_t t) =
-  { f_BITS = mk_u32 (bits t); f_SIGNED = signed t }
+  { f_bits = (fun () -> mk_u32 (bits t));
+    f_bits_pre = (fun () -> True);
+    f_bits_post = (fun () r -> r == mk_u32 (bits t));
+    f_SIGNED = signed t }
 "
 )]
 const _: () = {};
@@ -110,7 +116,7 @@ impl Bit {
         if x >= 0 {
             Self::of_raw_int(x as u128, nth)
         } else {
-            Self::of_raw_int((2i128.pow(T::BITS) + x) as u128, nth)
+            Self::of_raw_int((2i128.pow(T::bits()) + x) as u128, nth)
         }
     }
 }
