fstar-helpers/minicore/proofs/fstar/extraction/Minicore.Abstractions.Bitvec.fst
@@ -3,6 +3,13 @@ module Minicore.Abstractions.Bitvec
 open Core
 open FStar.Mul
 
+let _ =
+  (* This module has implicit dependencies, here we make them explicit. *)
+  (* The implicit dependencies arise from typeclasses instances. *)
+  let open Minicore.Abstractions.Bit in
+  let open Minicore.Abstractions.Funarr in
+  ()
+
 noeq
 
 /// A fixed-size bit vector type.
@@ -59,6 +66,95 @@ let impl_6 (v_N: usize) : Core.Ops.Index.t_Index (t_BitVec v_N) usize =
     fun (self: t_BitVec v_N) (index: usize) ->
       Minicore.Abstractions.Funarr.impl_6__get v_N #Minicore.Abstractions.Bit.t_Bit self._0 index
   }
+
+/// Convert a fun array of bits into an unsigned number.
+let math_int_from_fnarr_bit
+      (v_N: usize)
+      (bits: Minicore.Abstractions.Funarr.t_FunArray v_N Minicore.Abstractions.Bit.t_Bit)
+    : Hax_lib.Int.t_Int =
+  Minicore.Abstractions.Funarr.impl_6__fold v_N
+    #Minicore.Abstractions.Bit.t_Bit
+    #Hax_lib.Int.t_Int
+    bits
+    (0 <: Hax_lib.Int.t_Int)
+    (fun acc n ->
+        let acc:Hax_lib.Int.t_Int = acc in
+        let n:Minicore.Abstractions.Bit.t_Bit = n in
+        (acc * (2 <: Hax_lib.Int.t_Int) <: Hax_lib.Int.t_Int) +
+        (Rust_primitives.Hax.Int.from_machine (Core.Convert.f_from #u8
+                #Minicore.Abstractions.Bit.t_Bit
+                #FStar.Tactics.Typeclasses.solve
+                n
+              <:
+              u8)
+          <:
+          Hax_lib.Int.t_Int)
+        <:
+        Hax_lib.Int.t_Int)
+
+/// Convert a bit slice into a machine integer of type `T`.
+let int_from_fnarr_bit
+      (v_N: usize)
+      (#v_T: Type0)
+      (#[FStar.Tactics.Typeclasses.tcresolve ()] i1: Minicore.Abstractions.Bit.t_MachineInteger v_T)
+      (#[FStar.Tactics.Typeclasses.tcresolve ()] i2: Core.Marker.t_Copy v_T)
+      (bits: Minicore.Abstractions.Funarr.t_FunArray v_N Minicore.Abstractions.Bit.t_Bit)
+    : Prims.Pure Hax_lib.Int.t_Int
+      (requires
+        (Rust_primitives.Hax.Int.from_machine v_N <: Hax_lib.Int.t_Int) =
+        (Rust_primitives.Hax.Int.from_machine (Minicore.Abstractions.Bit.f_bits #v_T
+                #FStar.Tactics.Typeclasses.solve
+                ()
+              <:
+              u32)
+          <:
+          Hax_lib.Int.t_Int))
+      (fun _ -> Prims.l_True) =
+  let _:Prims.unit =
+    if true
+    then
+      let _:Prims.unit =
+        Hax_lib.v_assert (v_N =.
+            (cast (Minicore.Abstractions.Bit.f_bits #v_T #FStar.Tactics.Typeclasses.solve () <: u32)
+              <:
+              usize)
+            <:
+            bool)
+      in
+      ()
+  in
+  if Minicore.Abstractions.Bit.f_SIGNED #v_T #FStar.Tactics.Typeclasses.solve
+  then
+    let is_negative:bool =
+      match
+        bits.[ (cast (Minicore.Abstractions.Bit.f_bits #v_T #FStar.Tactics.Typeclasses.solve ()
+                <:
+                u32)
+            <:
+            usize) -!
+          mk_usize 1
+          <:
+          usize ]
+        <:
+        Minicore.Abstractions.Bit.t_Bit
+      with
+      | Minicore.Abstractions.Bit.Bit_One  -> true
+      | _ -> false
+    in
+    let s:Hax_lib.Int.t_Int =
+      math_int_from_fnarr_bit v_N
+        (Minicore.Abstractions.Funarr.impl_6__from_fn v_N
+            #Minicore.Abstractions.Bit.t_Bit
+            (fun i ->
+                let i:usize = i in
+                if i =. (v_N -! mk_usize 1 <: usize) <: bool
+                then Minicore.Abstractions.Bit.Bit_Zero <: Minicore.Abstractions.Bit.t_Bit
+                else bits.[ i ] <: Minicore.Abstractions.Bit.t_Bit)
+          <:
+          Minicore.Abstractions.Funarr.t_FunArray v_N Minicore.Abstractions.Bit.t_Bit)
+    in
+    if is_negative then (0 <: Hax_lib.Int.t_Int) - s else s
+  else math_int_from_fnarr_bit v_N bits
 
 let impl_7__from_fn
     (v_N: usize)
